\documentclass[10pt,a4paper]{article}
\usepackage[utf8]{inputenc}
\usepackage{amsmath}
\usepackage{amsfonts}
\usepackage{amssymb}
\usepackage{hyperref}
\author{Andrei Cristian\\\url{mailto:andrei.cristian1@info.uaic.ro}}
\title{Lab 1 - Exercise 6}
\begin{document}
\maketitle
\section{Definition of bisimulation}
A relation $Z \subseteq W \times W'$ is said to be \textit{bisimulation} between $M$ and $M'$ if the following conditions are satisfied:
\begin{enumerate}
\item For all $w \in W$ and $w' \in W'$ such that $(w, w') \in Z$ and each $p \in AP$, it holds $p \in L(w)$ if and only if $p \in L'(w')$;
\item If $(w, w') \in Z$ and $(w, v) \in R$, then there exists $v' \in W'$ such that $(v, v') \in Z$ and $(w', v') \in R'$ (\textit{forth condition});
\item If $(w, w') \in Z$ and $(w', v') \in R$, then there exists $v \in W$ such that $(v, v') \in Z$ and $(w, v) \in R$ (\textit{back condition}).
\end{enumerate}

Two worlds $w$ and $w'$ are called bisimilar, $w \leftrightsquigarrow_{M, M'} w'$, if there is  a bisimulation $Z$ between $M$ and $M'$ with $(w, w') \in Z$.

\section{Proposition 1}
Let $M = <W, R, L>$ and $M'=<W', R', L'>$ be two Kripke structures. Let $w \in W'$ such as $w \leftrightsquigarrow_{M, M'} w'$.Then $w$ and $w'$ are modally equivalent, i.e., for each formula Modal Logic $\varphi$,
	\[
	M, w \models \varphi \textrm{ iff. } M', w' \models \varphi
	\]
\section{Structural induction proof}

Demonstration using structural induction:

\begin{itemize}

\item
\begin{tabbing}
$\varphi = p \in AP$, \= $M, w \models p$ iff. $p \in L(w)$\\
\> $w\leftrightsquigarrow_{M, M'}w' \xrightarrow{1.} L(w) = L(w') \Rightarrow p \in L(w') \Rightarrow M', w' \models p$; \textbf{(a)}\\
\> $M', w' \models p$ iff. $p \in L(w')$\\
\> $w\leftrightsquigarrow_{M, M'}w' \xrightarrow{1.} L(w') = L(w) \Rightarrow p \in L(w) \Rightarrow M, w \models p$; \textbf{(b)}\\
\> $(a),(b)\Rightarrow M, w \models p$ iff. $M, w' \models p$.\\
$\Rightarrow M, w \models p$ iff. $M', w' \models p$.
\end{tabbing}
\item
\begin{tabbing}
$\varphi = \neg \varphi_1$, \= $M, w \models \neg \varphi_1$ iff. $M, w \not \models \varphi_1$; \textbf{(a)}\\
\> $M, w \models \varphi_1$ iff. $M', w' \models \varphi_1$; \textbf{(b)} -- demonstrated previously\\
\> $(a), (b) \Rightarrow M', w' \not \models \varphi_1 \Rightarrow M', w' \models \neg \varphi_1$.\\
\> $M', w' \models \neg \varphi_1$ iff. $M', w' \not \models \varphi_1$; \textbf{(c)}\\
\> $M', w' \models \varphi_1$ iff. $M, w \models \varphi_1$; \textbf{(d)} -- demonstrated previously\\
\> $(c), (d) \Rightarrow M, w \not \models \varphi_1 \Rightarrow M, w \models \neg \varphi_1$.\\
$\Rightarrow M, w \models \varphi$ iff. $M', w' \models \varphi$.
\end{tabbing}
\item
\begin{tabbing}
$\varphi = \lozenge \varphi_1$, \= $M, w \models \lozenge \varphi_1$ iff. $\exists t \in W, (w, t) \in R, M, t \models \varphi_1$; \textbf{(a)}\\
\> $w\leftrightsquigarrow_{M, M'} w' \xrightarrow{2.}$ if exists $(w, t) \in R$, then $\exists t' \in W', (w', t') \in R'$\\
\> and $t \leftrightsquigarrow_{M, M'} t'$; \textbf{(b)}\\
\> $(a), (b) \xrightarrow{IH} \exists t',(w', t') \in R', M', t' \models \varphi_1 \Rightarrow M', w' \models \lozenge \varphi_1$;\\
\> $M', w' \models \lozenge \varphi_1$ iff. $\exists t' \in W', (w', t') \in R', M', t' \models \varphi_1$; \textbf{(c)}\\
\> $w \leftrightsquigarrow_{M, M'} w' \xrightarrow{3.}$ if exists $(w', t') \in R'$, then $\exists t \in W, (w, t) \in R$\\
\> and $t \leftrightsquigarrow_{M, M'} t'$; \textbf{(d)}\\
\> $(c), (d) \xrightarrow{IH} \exists t, (w, t) \in R, M, t \models \varphi_1 \Rightarrow M, w \models \lozenge \varphi_1$.\\
$\Rightarrow M, w \models \varphi$ iff. $M', w' \models \varphi$.
\end{tabbing}
\item
\begin{tabbing}
$\varphi = \square \varphi_1$, \= $M, w \models \square \varphi_1$ iff. $\forall t \in W, (w, t) \in R, M, t \models \varphi_1$; \textbf{(a)}\\
\> $w \leftrightsquigarrow_{M, M'} w' \xrightarrow{2.}$ if exists $(w, t) \in R$, then $\exists t' \in W', (w', t') \in R'$\\
\> and $t \leftrightsquigarrow_{M, M'} t'$; \textbf{(b)}\\
\> $(a), (b) \xrightarrow{IH} \forall t', (w', t') \in R', M', t' \models \varphi_1 \Rightarrow M', w' \models \square \varphi_1$;\\
\> $M', w' \models \square \varphi_1$ iff. $\forall t' \in W', (w', t') \in R', M', t' \models \varphi_1$; \textbf{(c)}\\
\> $w \leftrightsquigarrow_{M, M'} w' \xrightarrow{3.}$ if exists $(w', t') \in R'$, then $\exists t \in W, (w, t) \in R$\\
\> and $t \leftrightsquigarrow_{M, M'} t'$; \textbf{(d)}\\
\> $(c), (d) \xrightarrow{IH} \forall t, (w, t) \in R, M, t \models \varphi_1 \Rightarrow M, w \models \square \varphi_1$.\\
$\Rightarrow M, w \models \varphi$ iff. $M', w' \models \varphi$.
\end{tabbing}
\end{itemize}

In conclusion, $\forall \varphi \in$ \textit{BML}, $M, w \models \varphi$ iff. $M', w' \models \varphi$

\end{document}